Updates to convergence concepts for potential infinite-valued r.v.'s

src/real/analysis/real_topologyScript.sml
@@ -106,117 +106,6 @@ val BIGUNION_MONO = store_thm ("BIGUNION_MONO",
  *)
 
 (* ------------------------------------------------------------------------- *)
-(* Metric function for R^1.                                                  *)
-(* ------------------------------------------------------------------------- *)
-
-(* new definition based on metricTheory *)
-Definition dist_def :
-    Dist = dist mr1
-End
-
-(* old definition (now becomes a theorem) *)
-Theorem dist :
-    !x y. Dist(x:real,y:real) = abs(x - y)
-Proof
-    RW_TAC std_ss [dist_def, MR1_DEF]
- >> REAL_ARITH_TAC
-QED
-
-val _ = overload_on ("dist",``Dist``);
-
-val DIST_REFL = store_thm ("DIST_REFL",
- ``!x. dist(x,x) = &0``,
-  SIMP_TAC std_ss [dist] THEN REAL_ARITH_TAC);
-
-val DIST_SYM = store_thm ("DIST_SYM",
- ``!x y. dist(x,y) = dist(y,x)``,
-  SIMP_TAC std_ss [dist] THEN REAL_ARITH_TAC);
-
-val DIST_TRIANGLE = store_thm ("DIST_TRIANGLE",
- ``!x:real y z. dist(x,z) <= dist(x,y) + dist(y,z)``,
-  SIMP_TAC std_ss [dist] THEN REAL_ARITH_TAC);
-
-val DIST_TRIANGLE_ALT = store_thm ("DIST_TRIANGLE_ALT",
- ``!x y z. dist(y,z) <= dist(x,y) + dist(x,z)``,
-  SIMP_TAC std_ss [dist] THEN REAL_ARITH_TAC);
-
-val DIST_EQ_0 = store_thm ("DIST_EQ_0",
- ``!x y. (dist(x,y) = 0:real) <=> (x = y)``,
-  SIMP_TAC std_ss [dist] THEN REAL_ARITH_TAC);
-
-val DIST_POS_LT = store_thm ("DIST_POS_LT",
- ``!x y. ~(x = y) ==> &0 < dist(x,y)``,
-  SIMP_TAC std_ss [dist] THEN REAL_ARITH_TAC);
-
-val DIST_NZ = store_thm ("DIST_NZ",
- ``!x y. ~(x = y) <=> &0 < dist(x,y)``,
-  SIMP_TAC std_ss [dist] THEN REAL_ARITH_TAC);
-
-val DIST_TRIANGLE_LE = store_thm ("DIST_TRIANGLE_LE",
- ``!x y z e. dist(x,z) + dist(y,z) <= e ==> dist(x,y) <= e``,
-  SIMP_TAC std_ss [dist] THEN REAL_ARITH_TAC);
-
-val DIST_TRIANGLE_LT = store_thm ("DIST_TRIANGLE_LT",
- ``!x y z e. dist(x,z) + dist(y,z) < e ==> dist(x,y) < e``,
-  SIMP_TAC std_ss [dist] THEN REAL_ARITH_TAC);
-
-val DIST_TRIANGLE_HALF_L = store_thm ("DIST_TRIANGLE_HALF_L",
- ``!x1 x2 y. dist(x1,y) < e / &2 /\ dist(x2,y) < e / &2 ==> dist(x1,x2) < e``,
-  REPEAT STRIP_TAC THEN KNOW_TAC `` dist (x1,y) + dist (x2,y) < e`` THENL
-  [METIS_TAC [REAL_LT_ADD2, REAL_HALF_DOUBLE],
-   DISCH_TAC THEN MATCH_MP_TAC REAL_LET_TRANS THEN
-   EXISTS_TAC ``dist (x1,y) + dist (x2,y)`` THEN
-   METIS_TAC [DIST_TRIANGLE, DIST_SYM]]);
-
-val DIST_TRIANGLE_HALF_R = store_thm ("DIST_TRIANGLE_HALF_R",
- ``!x1 x2 y. dist(y,x1) < e / &2 /\ dist(y,x2) < e / &2 ==> dist(x1,x2) < e``,
-  REPEAT STRIP_TAC THEN KNOW_TAC `` dist (y, x1) + dist (y, x2) < e`` THENL
-  [METIS_TAC [REAL_LT_ADD2, REAL_HALF_DOUBLE],
-   DISCH_TAC THEN MATCH_MP_TAC REAL_LET_TRANS THEN
-   EXISTS_TAC ``dist (y, x1) + dist (y, x2)`` THEN
-   METIS_TAC [DIST_TRIANGLE, DIST_SYM]]);
-
-val DIST_TRIANGLE_ADD = store_thm ("DIST_TRIANGLE_ADD",
- ``!x x' y y'. dist(x + y,x' + y') <= dist(x,x') + dist(y,y')``,
-  SIMP_TAC std_ss [dist] THEN REAL_ARITH_TAC);
-
-val DIST_MUL = store_thm ("DIST_MUL",
- ``!x y c. dist(c * x,c * y) = abs(c) * dist(x,y)``,
-  REWRITE_TAC[dist, GSYM ABS_MUL] THEN REAL_ARITH_TAC);
-
-val DIST_TRIANGLE_ADD_HALF = store_thm ("DIST_TRIANGLE_ADD_HALF",
- ``!x x' y y':real.
-    dist(x,x') < e / &2 /\ dist(y,y') < e / &2 ==> dist(x + y,x' + y') < e``,
-  REPEAT STRIP_TAC THEN KNOW_TAC `` dist (x, x') + dist (y, y') < e`` THENL
-  [METIS_TAC [REAL_LT_ADD2, REAL_HALF_DOUBLE],
-   DISCH_TAC THEN MATCH_MP_TAC REAL_LET_TRANS THEN
-   EXISTS_TAC ``dist (x, x') + dist (y, y')`` THEN
-   METIS_TAC [DIST_TRIANGLE_ADD, DIST_SYM]]);
-
-val DIST_LE_0 = store_thm ("DIST_LE_0",
- ``!x y. dist(x,y) <= &0 <=> (x = y)``,
-  SIMP_TAC std_ss [dist] THEN REAL_ARITH_TAC);
-
-val DIST_POS_LE = store_thm ("DIST_POS_LE",
- ``!x y. &0 <= dist(x,y)``,
-  METIS_TAC [DIST_EQ_0, DIST_NZ, REAL_LE_LT]);
-
-val DIST_EQ = store_thm ("DIST_EQ",
- ``!w x y z. (dist(w,x) = dist(y,z)) <=> (dist(w,x) pow 2 = dist(y,z) pow 2)``,
-  REPEAT GEN_TAC THEN EQ_TAC THENL [RW_TAC std_ss [],
-  DISCH_TAC THEN MATCH_MP_TAC POW_EQ THEN EXISTS_TAC ``1:num`` THEN
-  RW_TAC arith_ss [DIST_POS_LE]]);
-
-val DIST_0 = store_thm ("DIST_0",
- ``!x. (dist(x,0) = abs(x)) /\ (dist(0,x) = abs(x))``,
-  RW_TAC arith_ss [dist, REAL_SUB_RZERO, REAL_SUB_LZERO, ABS_NEG]);
-
-val REAL_CHOOSE_DIST = store_thm ("REAL_CHOOSE_DIST",
- ``!x e. &0 <= e ==> (?y. dist (x,y) = e)``,
-  REPEAT STRIP_TAC THEN EXISTS_TAC ``x - e:real`` THEN
-  ASM_REWRITE_TAC [dist, REAL_SUB_SUB2, ABS_REFL]);
-
-(* ------------------------------------------------------------------------- *)
 (* Linear functions.                                                         *)
 (* ------------------------------------------------------------------------- *)
 
@@ -4842,154 +4731,6 @@ val FRONTIER_INTER_SUBSET_INTER = store_thm ("FRONTIER_INTER_SUBSET_INTER",
    CLOSURE_INTER_SUBSET) THEN SET_TAC[]);
 
 (* ------------------------------------------------------------------------- *)
-(* A variant of nets (slightly non-standard but good for our purposes).      *)
-(* ------------------------------------------------------------------------- *)
-
-val isnet = new_definition("isnet",
- ``!g. isnet g = !x y. (!z. g z x ==> g z y) \/
-                       (!z. g z y ==> g z x)``);
-
-val net_tydef = new_type_definition
- ("net",
-  prove (``?(g:'a->'a->bool). isnet g``,
-        EXISTS_TAC ``\x:'a y:'a. F`` THEN REWRITE_TAC[isnet]));
-
-val net_ty_bij = define_new_type_bijections
-    {name="net_tybij",
-     ABS="mk_net", REP="netord",tyax=net_tydef};
-
-Theorem net_tybij[allow_rebind]:
-  (!a. mk_net (netord a) = a) /\
-  (!r. (!x y. (!z. r z x ==> r z y) \/ (!z. r z y ==> r z x)) <=>
-       (netord (mk_net r) = r))
-Proof
-  SIMP_TAC std_ss [net_ty_bij, GSYM isnet]
-QED
-
-val NET = store_thm ("NET",
- ``!n x y. (!z. netord n z x ==> netord n z y) \/
-           (!z. netord n z y ==> netord n z x)``,
-   REWRITE_TAC[net_tybij, ETA_AX]);
-
-val OLDNET = store_thm ("OLDNET",
- ``!n x y. netord n x x /\ netord n y y
-           ==> ?z. netord n z z /\
-                   !w. netord n w z ==> netord n w x /\ netord n w y``,
-  MESON_TAC[NET]);
-
-val NET_DILEMMA = store_thm ("NET_DILEMMA",
- ``!net. (?a. (?x. netord net x a) /\ (!x. netord net x a ==> P x)) /\
-         (?b. (?x. netord net x b) /\ (!x. netord net x b ==> Q x))
-         ==> ?c. (?x. netord net x c) /\ (!x. netord net x c ==> P x /\ Q x)``,
-  MESON_TAC[NET]);
-
-(* connection to netsTheory *)
-Theorem DORDER_NET :
-    !n. dorder (netord n)
-Proof
-    RW_TAC std_ss [dorder, OLDNET]
-QED
-
-(* ------------------------------------------------------------------------- *)
-(* Common nets and the "within" modifier for nets.                           *)
-(* ------------------------------------------------------------------------- *)
-
-val _ = set_fixity "within" (Infix(NONASSOC, 450));
-val _ = set_fixity "in_direction" (Infix(NONASSOC, 450));
-
-(* new definition, making connection to netsTheory *)
-Definition at_def :
-    at z = mk_net (nets$tendsto (mr1,z))
-End
-
-(* old definition, now becomes an equivalent theorem *)
-Theorem at :
-    !a. at a = mk_net(\x y. &0 < dist(x,a) /\ dist(x,a) <= dist(y,a))
-Proof
-    RW_TAC std_ss [at_def]
- >> AP_TERM_TAC
- >> RW_TAC std_ss [FUN_EQ_THM, tendsto, dist_def]
- >> PROVE_TAC [METRIC_SYM]
-QED
-
-val at_infinity = new_definition ("at_infinity",
-  ``at_infinity = mk_net(\x y. abs(x) >= abs(y))``);
-
-val at_posinfinity = new_definition ("at_posinfinity",
-  ``at_posinfinity = mk_net(\x y:real. x >= y)``);
-
-val at_neginfinity = new_definition ("at_neginfinity",
-  ``at_neginfinity = mk_net(\x y:real. x <= y)``);
-
-val sequentially = new_definition ("sequentially",
-  ``sequentially = mk_net(\m:num n. m >= n)``);
-
-val within = new_definition ("within",
-  ``(net within s) = mk_net(\x y. netord net x y /\ x IN s)``);
-
-val in_direction = new_definition ("in_direction",
-  ``(a in_direction v) = ((at a) within {b | ?c. &0 <= c /\ (b - a = c * v)})``);
-
-(* ------------------------------------------------------------------------- *)
-(* Prove that they are all nets.                                             *)
-(* ------------------------------------------------------------------------- *)
-
-fun NET_PROVE_TAC [def] =
-  SIMP_TAC std_ss [GSYM FUN_EQ_THM, def] THEN
-  REWRITE_TAC [ETA_AX] THEN
-  ASM_SIMP_TAC std_ss [GSYM(CONJUNCT2 net_tybij)];
-
-val AT = store_thm ("AT",
- ``!a:real x y.
-        netord(at a) x y <=> &0 < dist(x,a) /\ dist(x,a) <= dist(y,a)``,
-  GEN_TAC THEN NET_PROVE_TAC[at] THEN
-  METIS_TAC[REAL_LE_TOTAL, REAL_LE_REFL, REAL_LE_TRANS, REAL_LET_TRANS]);
-
-val AT_INFINITY = store_thm ("AT_INFINITY",
- ``!x y. netord at_infinity x y <=> abs(x) >= abs(y)``,
-  NET_PROVE_TAC[at_infinity] THEN
-  REWRITE_TAC[real_ge, REAL_LE_REFL] THEN
-  MESON_TAC[REAL_LE_TOTAL, REAL_LE_REFL, REAL_LE_TRANS]);
-
-val AT_POSINFINITY = store_thm ("AT_POSINFINITY",
- ``!x y. netord at_posinfinity x y <=> x >= y``,
-  NET_PROVE_TAC[at_posinfinity] THEN
-  REWRITE_TAC[real_ge, REAL_LE_REFL] THEN
-  MESON_TAC[REAL_LE_TOTAL, REAL_LE_REFL, REAL_LE_TRANS]);
-
-val AT_NEGINFINITY = store_thm ("AT_NEGINFINITY",
- ``!x y. netord at_neginfinity x y <=> x <= y``,
-  NET_PROVE_TAC[at_neginfinity] THEN
-  REWRITE_TAC[real_ge, REAL_LE_REFL] THEN
-  MESON_TAC[REAL_LE_TOTAL, REAL_LE_REFL, REAL_LE_TRANS]);
-
-val SEQUENTIALLY = store_thm ("SEQUENTIALLY",
- ``!m n. netord sequentially m n <=> m >= n``,
-  NET_PROVE_TAC[sequentially] THEN REWRITE_TAC[GREATER_EQ, LESS_EQ_REFL] THEN
-  MESON_TAC[LESS_EQ_CASES, LESS_EQ_REFL, LESS_EQ_TRANS]);
-
-val WITHIN = store_thm ("WITHIN",
- ``!n s x y. netord(n within s) x y <=> netord n x y /\ x IN s``,
-  GEN_TAC THEN GEN_TAC THEN SIMP_TAC std_ss [within, GSYM FUN_EQ_THM] THEN
-  REWRITE_TAC[GSYM(CONJUNCT2 net_tybij), ETA_AX] THEN
-  METIS_TAC[NET]);
-
-val IN_DIRECTION = store_thm ("IN_DIRECTION",
- ``!a v x y. netord(a in_direction v) x y <=>
-                &0 < dist(x,a) /\ dist(x,a) <= dist(y,a) /\
-                 ?c. &0 <= c /\ (x - a = c * v)``,
-  SIMP_TAC std_ss [WITHIN, AT, in_direction, GSPECIFICATION] THEN METIS_TAC []);
-
-val WITHIN_UNIV = store_thm ("WITHIN_UNIV",
- ``!x:real. (at x within UNIV) = at x``,
-  REWRITE_TAC[within, at, IN_UNIV] THEN REWRITE_TAC[ETA_AX, net_tybij]);
-
-val WITHIN_WITHIN = store_thm ("WITHIN_WITHIN",
- ``!net s t. ((net within s) within t) = (net within (s INTER t))``,
-  ONCE_REWRITE_TAC[within] THEN
-  REWRITE_TAC[WITHIN, IN_INTER, GSYM CONJ_ASSOC]);
-
-(* ------------------------------------------------------------------------- *)
 (* Identify trivial limits, where we can't approach arbitrarily closely.     *)
 (* ------------------------------------------------------------------------- *)
 
@@ -5206,14 +4947,15 @@ val FORALL_EVENTUALLY = store_thm ("FORALL_EVENTUALLY",
 (* Limits, defined as vacuously true when the limit is trivial.              *)
 (* ------------------------------------------------------------------------- *)
 
-val _ = hide "-->";
-
 (* NOTE: This is for (f :'a -> real) (l :real) (net :'a net).
          Now the name "tendsto_real" follows HOL-Light's "realanalysis.ml".
  *)
-val tendsto_real = new_infixr_definition
-  ("tendsto_real",
-  ``$--> f l net = !e. &0 < e ==> eventually (\x. dist(f(x),l) < e) net``,750);
+Definition tendsto_real :
+    tendsto_real f l net <=> !e. &0 < e ==> eventually (\x. dist(f(x),l) < e) net
+End
+
+Overload "-->" = “tendsto_real”
+val _ = set_fixity "-->" (Infixr 750);
 
 val tendsto = tendsto_real;
 
@@ -8564,11 +8306,19 @@ val CONTINUOUS_WITHIN_COMPARISON = store_thm ("CONTINUOUS_WITHIN_COMPARISON",
 val _ = set_fixity "continuous_on" (Infix(NONASSOC, 450));
 val _ = set_fixity "uniformly_continuous_on" (Infix(NONASSOC, 450));
 
-val continuous_on = new_definition ("continuous_on",
- ``f continuous_on s <=>
-   !x. x IN s ==> !e. &0 < e
-   ==> ?d. &0 < d /\ !x'. x' IN s /\ dist(x',x) < d
-     ==> dist(f(x'),f(x)) < e``);
+Definition continuous_on_def :
+    f continuous_on s <=> !x. x IN s ==> f continuous (at x within s)
+End
+Theorem CONTINUOUS_ON_EQ_CONTINUOUS_WITHIN = continuous_on_def
+
+Theorem continuous_on :
+    !f s. f continuous_on s <=>
+          !x. x IN s ==> !e. &0 < e
+                     ==> ?d. &0 < d /\ !x'. x' IN s /\ dist(x',x) < d
+                                             ==> dist(f(x'),f(x)) < e
+Proof
+    rw [continuous_on_def, continuous_within]
+QED
 
 val uniformly_continuous_on = new_definition ("uniformly_continuous_on",
  ``f uniformly_continuous_on s <=>
@@ -8587,10 +8337,6 @@ val UNIFORMLY_CONTINUOUS_IMP_CONTINUOUS = store_thm ("UNIFORMLY_CONTINUOUS_IMP_C
 val CONTINUOUS_AT_IMP_CONTINUOUS_ON = store_thm ("CONTINUOUS_AT_IMP_CONTINUOUS_ON",
  ``!f s. (!x. x IN s ==> f continuous (at x)) ==> f continuous_on s``,
   REWRITE_TAC[continuous_at, continuous_on] THEN MESON_TAC[]);
-
-val CONTINUOUS_ON_EQ_CONTINUOUS_WITHIN = store_thm ("CONTINUOUS_ON_EQ_CONTINUOUS_WITHIN",
- ``!f s. f continuous_on s <=> !x. x IN s ==> f continuous (at x within s)``,
- REWRITE_TAC[continuous_on, continuous_within]);
 
 val CONTINUOUS_ON = store_thm ("CONTINUOUS_ON",
  ``!f (s:real->bool).
